[Progress] Port layers to weakest precondition style reasoning.

src/Framework/Simulation/WeakestPreconditions.v
@@ -2,6 +2,61 @@ Require Import List Primitives Layer Simulation.Definitions.
 
 (* WP reasoning for proving bisimulations *)
 
+Section OperationWP.
+Import Operation.
+
+Definition wp_low_to_high_op {low high: Operation}
+           (refines_to: low.(state) -> high.(state) -> Prop)
+           (compilation_of: forall T, low.(prog) T -> high.(prog) T -> Prop)
+           (oracle_refines_to : forall T, low.(state) -> high.(prog) T -> low.(oracle) -> high.(oracle) -> Prop) :=
+  forall T o1 o2 s1 s2 s1' v p1 p2,
+     low.(weakest_precondition) p1  (fun r s => exists s2', refines_to s s2' /\ r = v) o1 s1 ->
+     compilation_of T p1 p2 ->
+     refines_to s1 s2 ->
+     oracle_refines_to T s1 p2 o1 o2 ->
+     low.(exec) o1 s1 p1 (Finished s1' v) ->
+     high.(weakest_precondition) p2 (fun r s => refines_to s1' s /\ r = v) o2 s2.
+
+Definition wpc_low_to_high_op {low high: Operation}
+           (refines_to: low.(state) -> high.(state) -> Prop)
+           (compilation_of: forall T, low.(prog) T -> high.(prog) T -> Prop)
+           (oracle_refines_to : forall T, low.(state) -> high.(prog) T -> low.(oracle) -> high.(oracle) -> Prop) :=
+  forall T o1 o2 s1 s2 s1' p1 p2,
+     low.(weakest_crash_precondition) p1 (fun s => exists s2', refines_to s s2') o1 s1 ->
+     compilation_of T p1 p2 ->
+     refines_to s1 s2 ->
+     oracle_refines_to T s1 p2 o1 o2 ->
+     low.(exec) o1 s1 p1 (Crashed s1') ->
+     high.(weakest_crash_precondition) p2 (fun s => refines_to s1' s) o2 s2.
+
+Definition wp_high_to_low_op {low high: Operation}
+           (refines_to: low.(state) -> high.(state) -> Prop)
+           (compilation_of: forall T, low.(prog) T -> high.(prog) T -> Prop)
+           (oracle_refines_to : forall T, low.(state) -> high.(prog) T -> low.(oracle) -> high.(oracle) -> Prop) :=
+  forall T o1 o2 s1 s2 s2' v p1 p2,
+     high.(weakest_precondition) p2 (fun r s => exists s1', refines_to s1' s /\ r = v) o2 s2 ->
+     compilation_of T p1 p2 ->
+     refines_to s1 s2 ->
+     oracle_refines_to T s1 p2 o1 o2 ->
+     high.(exec) o2 s2 p2 (Finished s2' v) ->
+     low.(weakest_precondition) p1 (fun r s => refines_to s s2' /\ r = v) o1 s1.
+
+Definition wpc_high_to_low_op {low high: Operation}
+           (refines_to: low.(state) -> high.(state) -> Prop)
+           (compilation_of: forall T, low.(prog) T -> high.(prog) T -> Prop)
+           (oracle_refines_to : forall T, low.(state) -> high.(prog) T -> low.(oracle) -> high.(oracle) -> Prop) :=
+  forall T o1 o2 s1 s2 s2' p1 p2,
+    high.(weakest_crash_precondition) p2 (fun s => exists s1', refines_to s1' s) o2 s2 ->
+    compilation_of T p1 p2 ->
+    refines_to s1 s2 ->
+    oracle_refines_to T s1 p2 o1 o2 ->
+    high.(exec) o2 s2 p2 (Crashed s2') ->
+    low.(weakest_crash_precondition) p1 (fun s => refines_to s s2') o1 s1.
+
+End OperationWP.
+
+Section LanguageWP.
+
 Definition wp_low_to_high {O1 O2} {low: Language O1} {high: Language O2}
            (refines_to: low.(state) -> high.(state) -> Prop)
            (compilation_of: forall T, low.(prog) T -> high.(prog) T -> Prop)
@@ -49,3 +104,96 @@ Definition wpc_high_to_low {O1 O2} {low: Language O1} {high: Language O2}
     oracle_refines_to T s1 p2 o1 o2 ->
     high.(exec) o2 s2 p2 (Crashed s2') ->
     low.(weakest_crash_precondition) p1 (fun s => refines_to s s2') o1 s1.
+
+End LanguageWP.
+
+Section OperationToLanguageWP.
+  
+  Fixpoint lift_compilation_of {O1 O2} {L1: Language O1} {L2: Language O2}
+             (compilation_of: forall T, O1.(Operation.prog) T -> O2.(Operation.prog) T -> Prop)
+             T (p1: L1.(prog) T) (p2: L2.(prog) T) : Prop.
+    destruct p2.
+    (* Op *)
+    - exact (exists p1', p1 = Op _ _ p1' /\ compilation_of T p1' p).
+    (* Ret *)
+    - exact (p1 = Ret t).
+    (* Bind *)
+    - exact (exists px1 py1,
+               p1 = Bind px1 py1 /\
+               lift_compilation_of O1 O2 L1 L2 compilation_of T px1 p2 /\
+               (forall r, lift_compilation_of O1 O2 L1 L2 compilation_of T' (py1 r) (p r))).
+  Defined.
+
+  Fixpoint lift_oracle_refines_to {O1 O2} {L1: Language O1} {L2: Language O2}
+           (compilation_of: forall T, O1.(Operation.prog) T -> O2.(Operation.prog) T -> Prop)
+           (oracle_refines_to : forall T, O1.(Operation.state) -> O2.(Operation.prog) T ->
+                                     O1.(Operation.oracle) -> O2.(Operation.oracle) -> Prop)
+           T (s1 : L1.(state)) (p2: L2.(prog) T) (o1 : L1.(oracle)) (o2: L2.(oracle)) : Prop :=
+    match p2 with
+    | Op _ _ p2' =>
+      exists o1' o2',
+      o1 = [OpOracle _ o1'] /\
+      o2 = [OpOracle _ o2'] /\
+      oracle_refines_to _ s1 p2' o1' o2'
+    | Ret _ =>
+      (o1 = [Cont _] /\ o2 = [Cont _]) \/
+      (o1 = [Crash _] /\ o2 = [Crash _])
+    | @Bind _ T' T'' px py =>
+      exists o1' o1'' o2' o2'',
+      o1 = o1'++o1'' /\
+      o2 = o2'++o2'' /\
+      @lift_oracle_refines_to O1 O2 L1 L2 compilation_of oracle_refines_to _ s1 px o1' o2' /\
+      (forall px1,
+         @lift_compilation_of O1 O2 L1 L2 compilation_of _ px1 px ->
+         forall s1' r,
+           L1.(exec) o1' s1 px1 (Finished s1' r) ->
+           @lift_oracle_refines_to O1 O2 L1 L2 compilation_of oracle_refines_to _ s1' (py r) o1'' o2'')
+    end.
+      
+    
+  Theorem  wp_low_to_high_op_to_lang :
+           forall (O_low O_high: Operation) (low: Language O_low) (high: Language O_high)
+           (refines_to: O_low.(Operation.state) -> O_high.(Operation.state) -> Prop)
+           (compilation_of: forall T, O_low.(Operation.prog) T -> O_high.(Operation.prog) T -> Prop)
+           (oracle_refines_to : forall T, O_low.(Operation.state) -> O_high.(Operation.prog) T ->
+                                     O_low.(Operation.oracle) -> O_high.(Operation.oracle) -> Prop),
+
+             wp_low_to_high_op refines_to compilation_of oracle_refines_to ->
+             @wp_low_to_high O_low O_high low high refines_to (lift_compilation_of compilation_of) (lift_oracle_refines_to compilation_of oracle_refines_to).
+  Proof.
+    unfold wp_low_to_high_op, wp_low_to_high; intros.
+
+    generalize dependent o1;
+    generalize dependent o2;
+    generalize dependent s1;
+    generalize dependent s2;
+    generalize dependent s1';
+    generalize dependent v;
+    generalize dependent p1;
+    generalize dependent p2.
+    induction p2; simpl in *; intros; cleanup; invert_exec.
+    { (* Op *)
+      inversion H0; cleanup; eauto.
+    }
+    {(* Ret *)
+      split_ors; cleanup; eauto.
+    }    
+    {(* Bind *)
+      clear H.
+      simpl in *; cleanup.
+      
+      do 2 eexists; split; eauto.
+      eapply wp_complete; intros; eauto.
+      instantiate (1:= fun o s => exists s' r, exec high o s p2 (Finished s' r) /\ refines_to x7 s' /\ r = x8) in X.
+      simpl in *; cleanup.
+      
+      do 2 eexists; split; eauto.
+      eapply H0.
+      eauto.
+      eauto.
+      admit.
+      eapply H8; eauto.
+      (* TODO: Maybe finish these transfer lemmas? *)
+  Abort.
+  
+End OperationToLanguageWP.
