src/Layers/LoggedDiskLayer/Definitions.v
@@ -43,7 +43,62 @@ Set Implicit Arguments.
       forall d la lv,
         exec [CrashAfter] d (Write la lv) (Crashed (write_all d la lv)).
 
-  Hint Constructors exec.
+  Hint Constructors exec : core.
+
+   Definition weakest_precondition T (p: prog T) :=
+   match p in prog T' return (T' -> state -> Prop) -> oracle -> state -> Prop with
+   | Read a =>
+     (fun Q o s =>
+       exists v,
+         o = [Cont] /\
+         read s a = Some v /\
+         Q v s)
+   | Write la lv =>
+     (fun Q o s =>
+       o = [Cont] /\
+       Q tt (write_all s la lv))
+   end.
+
+  Definition weakest_crash_precondition T (p: prog T) :=
+    match p in prog T' return (state -> Prop) -> oracle -> state -> Prop with
+   | Read a =>
+     (fun Q o s =>
+         o = [CrashBefore] /\
+         Q s)
+   | Write la lv =>
+     (fun Q o s =>
+       (o = [CrashBefore] /\
+        Q s) \/
+       (o = [CrashAfter] /\
+        Q (write_all s la lv)))
+   end.
+
+  Theorem wp_complete:
+    forall T (p: prog T) H Q,
+      (forall o s, H o s -> weakest_precondition p Q o s) <->
+      (forall o s, H o s -> (exists s' v, exec o s p (Finished s' v) /\ Q v s')).
+  Proof.
+    intros; destruct p; simpl; eauto;
+    split; intros;
+    specialize H0 with (1:= X);
+    cleanup; eauto;
+
+    inversion H0; cleanup; eauto.
+  Qed.
+  
+  Theorem wcp_complete:
+    forall T (p: prog T) H C,
+      (forall o s, H o s -> weakest_crash_precondition p C o s) <->
+      (forall o s, H o s -> (exists s', exec o s p (Crashed s') /\ C s')).
+  Proof.
+    unfold weakest_crash_precondition;
+    intros; destruct p; simpl; eauto;
+    split; intros;
+    specialize H0 with (1:= X);
+    cleanup; eauto;
+
+    inversion H0; cleanup; eauto.
+  Qed.
   
   Fixpoint oracle_ok T (p: prog T) o (s: state) :=
     match p with
@@ -80,22 +135,18 @@ Set Implicit Arguments.
       end; eauto.
   Qed.
   
-Module LoggedDiskOperation <: Operation.
-  Definition oracle := oracle.
-  Definition oracle_dec:= list_eq_dec token_dec.
-  Definition state := state.
-  Definition prog := prog.
-  Definition exec := exec.
-  Definition oracle_ok := oracle_ok.
-  Definition exec_deterministic_wrt_oracle :=
-    exec_deterministic_wrt_oracle.
-  Definition exec_then_oracle_ok :=
-    exec_then_oracle_ok.
-End LoggedDiskOperation.
+  Definition LoggedDiskOperation :=
+    Build_Operation
+      (list_eq_dec token_dec)
+      prog
+      exec
+      weakest_precondition
+      weakest_crash_precondition
+      wp_complete
+      wcp_complete
+      exec_deterministic_wrt_oracle.
 
-Module LoggedDiskHL := HoareLogic LoggedDiskOperation.
-Export LoggedDiskHL.
-
-Definition logged_disk_lts := Build_LTS LoggedDiskHL.Lang.oracle LoggedDiskHL.Lang.state LoggedDiskHL.Lang.prog LoggedDiskHL.Lang.exec.
+  Definition LoggedDiskLang := Build_Language LoggedDiskOperation.
+  Definition LoggedDiskHL := Build_HoareLogic LoggedDiskLang.
 
 Notation "p >> s" := (p s) (right associativity, at level 60, only parsing).
