src/Layers/CryptoDiskLayer/Definitions.v
@@ -1,0 +1,12 @@
+Require Import Framework.
+Require Import DiskLayer CryptoLayer.
+Import ListNotations.
+
+Set Implicit Arguments.
+
+Definition CryptoDiskOperation :=  HorizontalComposition CryptoOperation DiskOperation.
+Definition CryptoDiskLang := Build_Language CryptoDiskOperation.
+Definition CryptoDiskHL := Build_HoareLogic CryptoDiskLang.
+
+Notation "| p |" := (Language.Op CryptoDiskOperation _ p)(at level 60).
+Notation "x <-| p1 ; p2" := (Bind (Op CryptoDiskOperation _ p1) (fun x => p2))(right associativity, at level 60).
