src/Layers/CryptoLayer/Definitions.v
@@ -1,0 +1,161 @@
+Require Import Framework.
+Import ListNotations.
+
+Set Implicit Arguments.
+
+Instance value_eq_dec: EqDec value := value_dec.
+Instance hash_eq_dec: EqDec hash := hash_dec.
+
+Definition hashmap := @mem hash hash_dec (hash * value).
+Definition encryptionmap := @mem value value_dec (key * value).
+  
+  Inductive token :=
+  | Key : key -> token
+  | Crash : token
+  | Cont : token.
+
+  Definition token_dec : forall (t t': token), {t=t'}+{t<>t'}.
+    decide equality.
+    apply key_dec.
+  Defined.
+
+  Definition oracle := list token.
+
+  Definition state := ((list key * encryptionmap)* hashmap)%type.
+  
+  Inductive prog : Type -> Type :=
+  | GetKey : list value -> prog key
+  | Hash : hash -> value -> prog hash
+  | Encrypt : key -> value -> prog value
+  | Decrypt : key -> value -> prog value.
+   
+  Inductive exec :
+    forall T, oracle ->  state -> prog T -> @Result state T -> Prop :=
+
+  | ExecHash : 
+      forall em hm h v,
+        let hv := hash_function h v in
+        consistent hm hv (h, v) ->
+        exec [Cont] (em, hm) (Hash h v) (Finished (em, (upd hm hv (h, v))) hv)
+             
+  | ExecEncrypt : 
+      forall kl em hm k v,
+        let ev := encrypt k v in
+        consistent em ev (k, v) ->
+        exec [Cont] (kl, em, hm) (Encrypt k v) (Finished (kl, (upd em ev (k, v)), hm) ev)
+
+  | ExecDecrypt : 
+      forall kl em hm ev k v,
+        ev = encrypt k v ->
+        em ev = Some (k, v) ->
+        exec [Cont] (kl, em, hm) (Decrypt k ev) (Finished (kl, em, hm) v)
+
+  | ExecGetKey : 
+      forall vl kl em hm k,
+        ~In k kl ->
+        consistent_with_upds em
+             (map (encrypt k) vl) (map (fun v => (k, v)) vl) ->
+        exec [Key k] (kl, em, hm) (GetKey vl) (Finished ((k::kl), em, hm) k)
+ 
+  | ExecCrash :
+      forall T d (p: prog T),
+        exec [Crash] d p (Crashed d).
+
+  Hint Constructors exec : core.
+
+  Definition weakest_precondition T (p: prog T) :=
+    match p in prog T' return (T' -> state -> Prop) -> oracle -> state -> Prop with
+    | Hash h v =>
+      fun Q o s =>
+        let '(em, hm) := s in
+        o = [Cont] /\
+        let hv := hash_function h v in
+        consistent hm hv (h, v) /\
+        Q hv (em, (upd hm hv (h, v)))
+
+    | Encrypt k v => 
+      fun Q o s =>
+        let '(kl, em, hm) := s in
+        let ev := encrypt k v in
+        o = [Cont] /\
+        consistent em ev (k, v) /\
+        Q ev (kl, (upd em ev (k, v)), hm)
+
+    | Decrypt k ev => 
+      fun Q o s =>
+        let '(kl, em, hm) := s in
+        exists v,
+          o = [Cont] /\
+          ev = encrypt k v /\
+          em ev = Some (k, v) /\
+          Q v s
+          
+    | GetKey vl =>
+      fun Q o s =>
+        let '(kl, em, hm) := s in
+        (exists k,
+           o = [Key k] /\
+           ~In k kl /\
+           consistent_with_upds em (map (encrypt k) vl) (map (fun v => (k,v)) vl) /\
+           Q k ((k::kl), em, hm))
+    end.
+
+
+  Definition weakest_crash_precondition T (p: prog T) :=
+    fun Q o (s: state) => o = [Crash] /\ Q s.
+
+  Theorem exec_deterministic_wrt_oracle :
+    forall o s T (p: prog T) ret1 ret2,
+      exec o s p ret1 ->
+      exec o s p ret2 ->
+      ret1 = ret2.
+  Proof.
+    intros; destruct p; simpl in *; cleanup;
+    repeat
+      match goal with
+      | [H: exec _ _ _ _ |- _] =>
+        inversion H; clear H; cleanup
+      end; eauto.
+  Qed.
+
+  Theorem wp_complete:
+    forall T (p: prog T) H Q,
+      (forall o s, H o s -> weakest_precondition p Q o s) <->
+      (forall o s, H o s -> (exists s' v, exec o s p (Finished s' v) /\ Q v s')).
+  Proof.
+    intros; destruct p; simpl; eauto;
+    split; intros;
+    specialize H0 with (1:= X);
+    cleanup; eauto;
+    inversion H0; cleanup; eauto.
+  Qed.
+  
+  Theorem wcp_complete:
+    forall T (p: prog T) H C,
+      (forall o s, H o s -> weakest_crash_precondition p C o s) <->
+      (forall o s, H o s -> (exists s', exec o s p (Crashed s') /\ C s')).
+  Proof.
+    unfold weakest_crash_precondition;
+    intros; destruct p; simpl; eauto;
+    split; intros;
+    specialize H0 with (1:= X);
+    cleanup; eauto;
+    inversion H0; cleanup; eauto.
+  Qed.
+
+  
+  Definition CryptoOperation :=
+    Build_Operation
+      (list_eq_dec token_dec)
+      prog
+      exec
+      weakest_precondition
+      weakest_crash_precondition
+      wp_complete
+      wcp_complete
+      exec_deterministic_wrt_oracle.
+  
+  Definition CryptoLang := Build_Language CryptoOperation.
+  Definition CryptoHL := Build_HoareLogic CryptoLang.
+
+Notation "p >> s" := (p s) (right associativity, at level 60, only parsing).
