src/Layers/DiskLayer/Specs.v
@@ -1,9 +1,15 @@
+(*
 Require Import Framework.
 Require Import DiskLayer.Definitions.
 Open Scope pred_scope.
 
+
+Notation "| p |" := (Op DiskOperation _ p)(at level 60).
+
 Theorem read_ok:
   forall F o s a v,
+    LANG: DiskLang
+    LOGIC: DiskHL
     << o, s >>
     PRE:
      (F * a |-> v >> s)
@@ -11,25 +17,26 @@ Theorem read_ok:
      |Read a|
     << r, s' >>
     POST:
-     (F * a |-> v * [[r = fst v]] * [[fst s' = fst s]] >> s')
+     (F * a |-> v * [[r = fst v]] >> s')
     CRASH:
-     (F * a |-> v * [[fst s' = fst s]] >> s').
+     (F * a |-> v >> s').
 Proof.
   intros.
-  unfold hoare_triple; intros.
+  unfold hoare_triple, hoare_triple'; intros.
   destruct_lift H; cleanup.
   
   eapply ptsto_valid' in H0 as Hx;
     cleanup; eauto.  
-  split_ors.
+  
   eexists; intuition eauto;
   repeat econstructor; intuition eauto.
+  repeat econstructor; eauto.
   unfold read in *; cleanup; eauto.
   
   simpl in *; pred_apply; cancel; eauto.
 
   eexists; intuition eauto.
-  eapply ExecOpCrash; eauto;
+  eapply (ExecOpCrash _); eauto;
   econstructor; eauto.
   
   right; eexists; intuition eauto.
@@ -38,6 +45,8 @@ Qed.
 
 Theorem write_ok:
   forall F o s a v v',
+    LANG: DiskLang
+    LOGIC: DiskHL
     << o, s >>
      PRE: (F * a |-> v >> s)
      PROG: |Write a v'|
@@ -46,161 +55,29 @@ Theorem write_ok:
      CRASH: (F * a |-> v * [[fst s' = fst s]] >> s').
 Proof.
   intros.
-  unfold hoare_triple; intros.
+  unfold hoare_triple, hoare_triple'; intros.
   destruct_lift H; subst.
   eapply ptsto_valid' in H0 as Hx;
     cleanup; eauto.  
   split_ors.
   eexists; intuition eauto;
   repeat econstructor; intuition eauto.
+  repeat econstructor; eauto.
   
-    unfold read in *; cleanup; eauto.  
-    unfold write; cleanup.
-    unfold upd_disk; simpl.
-    eapply ptsto_upd' in H0; eauto.
-    pred_apply' H0; cancel.
-
-    eexists; intuition eauto.
-    eapply ExecOpCrash; eauto;
-    econstructor; eauto.
-    right; eexists; intuition eauto.
-    simpl in *; pred_apply; cancel; eauto.
-Qed.
-
-Theorem getkey_ok:
-  forall F vl o s,
-    let kl := fst (fst (fst s)) in
-    let em := snd (fst (fst s)) in
-    let hm := snd (fst s) in
-    << o, s >>
-     PRE: F >> s
-     PROG: |GetKey vl|
-    << r, s' >>
-     POST:
-      F * [[~In r kl]] *
-      [[consistent_with_upds em
-          (map (encrypt r) vl) (map (fun v => (r, v)) vl) ]] *
-      [[fst s' = (r::kl, em, hm)]] >> s'
-     CRASH:
-      (F * [[fst s' = fst s]] >> s') .
-Proof.
-  intros.
-  unfold hoare_triple; intros.
-  destruct s, p, p; simpl in *.
-  simpl in *; cleanup;
-  split_ors; eexists;
-    intuition eauto.
   
-  repeat econstructor; intuition eauto.
-  left; do 2 eexists; intuition eauto.
-  simpl in *; pred_apply; cancel; eauto.
-
-  eapply ExecOpCrash; econstructor; eauto.
+  unfold read in *; cleanup; intuition; cleanup.
+  unfold write; cleanup.
+  unfold upd_disk; simpl.
+  eapply ptsto_upd' in H0; eauto.
+  pred_apply' H0; cancel.
   
+  eexists; intuition eauto.
+  eapply (ExecOpCrash _); eauto;
+  econstructor; eauto.
   right; eexists; intuition eauto.
-  simpl; pred_apply; cancel.    
-Qed.  
-
-
-Theorem hash_ok:
-  forall F o s h v,
-    let hv := hash_function h v in
-    let kl := fst (fst (fst s)) in
-    let em := snd (fst (fst s)) in
-    let hm := snd (fst s) in
-    << o, s >>
-     PRE: (F * [[ consistent hm hv (h, v) ]] >> s)
-     PROG: (|Hash h v|)
-    << r, s' >>
-     POST: (F * [[r = hv]] * [[fst s' = (kl, em, upd hm hv (h, v))]] >> s')
-     CRASH: (F * [[fst s' = fst s]] >> s').
-Proof.
-  intros.
-  unfold hoare_triple; intros.
-  destruct s, p, p; simpl; intros.
-  destruct_lift H0;
-  simpl in *; cleanup; simpl in *.
-  split_ors; eexists;
-    intuition eauto.
-
-  do 2 econstructor; intuition eauto.
-  left; do 2 eexists; intuition eauto.
-  simpl; pred_apply; cancel; eauto.
-
-  
-  eapply ExecOpCrash; econstructor; eauto.
-  
-  simpl in *; cleanup; right; eexists; intuition eauto.
-  simpl; pred_apply; cancel.    
+  simpl in *; pred_apply; cancel; eauto.
 Qed.
 
-
-Theorem encrypt_ok:
-  forall F o s k v,
-    let ev := encrypt k v in
-    let kl := fst (fst (fst s)) in
-    let em := snd (fst (fst s)) in
-    let hm := snd (fst s) in
-    << o, s >>
-     PRE: (F * [[ consistent em ev (k, v) ]] >> s)
-     PROG: (|Encrypt k v|)
-    << r, s' >>
-     POST: (F * [[r = ev]] *
-                [[fst s' = (kl, upd em ev (k, v), hm)]] >> s')
-     CRASH: (F * [[fst s' = fst s]] >> s').
-Proof.
-  intros.
-  unfold hoare_triple; intros.
-  destruct s, p, p; simpl; intros.
-  destruct_lift H0; cleanup.
-  split_ors; eexists;
-  intuition eauto.
-
-  do 2 econstructor; intuition eauto.
-  
-  left; do 2 eexists; intuition eauto.
-  simpl; pred_apply; cancel; eauto.
-
-  eapply ExecOpCrash; econstructor; eauto.
-  
-  simpl in *; cleanup; right; eexists; intuition eauto.
-  simpl; pred_apply; cancel.    
-Qed.
-
-
-Theorem decrypt_ok:
-  forall F o s k ev v,
-    let kl := fst (fst (fst s)) in
-    let em := snd (fst (fst s)) in
-    let hm := snd (fst s) in
-    << o, s >>
-     PRE: (F * [[ ev = encrypt k v ]] * [[ em ev = Some (k, v) ]] >> s)
-     PROG: (|Decrypt k ev|)
-    << r, s' >>
-     POST: (F * [[r = v]] * [[fst s' = fst s]] >> s')
-     CRASH: (F * [[fst s' = fst s]] >> s').
-Proof.
-  intros.
-  unfold hoare_triple; intros.
-  destruct s, p, p; simpl; intros.
-  destruct_lift H0; cleanup.
-  split_ors; eexists;
-    intuition eauto.
-
-  do 2 econstructor; intuition eauto.
-  
-  left; do 2 eexists; intuition eauto.
-  simpl; pred_apply; cancel; eauto.
-
-  eapply ExecOpCrash; econstructor; eauto.
-  
-  simpl in *; cleanup; right; eexists; intuition eauto.
-  simpl; pred_apply; cancel.    
-Qed.
-
-Hint Extern 1 (hoare_triple _ _ (|Read _|) _ _ _ _ _ _) => eapply read_ok : specs.
-Hint Extern 1 (hoare_triple _ _ (|Write _ _|) _ _ _ _ _ _) => eapply write_ok : specs.
-Hint Extern 1 (hoare_triple _ _ (|Hash _ _|) _ _ _ _ _ _) => eapply hash_ok : specs.
-Hint Extern 1 (hoare_triple _ _ (|GetKey _|) _ _ _ _ _ _) => eapply getkey_ok : specs.
-Hint Extern 1 (hoare_triple _ _ (|Encrypt _ _|) _ _ _ _ _ _) => eapply encrypt_ok : specs.
-Hint Extern 1 (hoare_triple _ _ (|Decrypt _ _|) _ _ _ _ _ _) => eapply decrypt_ok : specs.
+Hint Extern 1 (hoare_triple _ _ _ (|Read _|) _ _ _ _ _ _) => eapply read_ok : specs.
+Hint Extern 1 (hoare_triple _ _ _ (|Write _ _|) _ _ _ _ _ _) => eapply write_ok : specs.
+*)
